\newcommand{\content}{$$
\inference[<]{\inference{\token{We}}{\cat{NP}:\mathrm{we}_{0}}\inference[>]{\inference{\token{found}}{(\cat{S} \bsl \cat{NP})/\cat{NP}:\lambda x.\lambda y.\mathrm{find}_{0}^{0}(x, y)}\inference[<]{\inference[>]{\inference{\token{the}}{\cat{NP}/\cat{N}:\lambda x.x}\inference{\token{service}}{\cat{N}:\mathrm{service}_{0}}}{\cat{NP}:\mathrm{service}_{0}}\inference{\inference[>]{\inference{\token{to}}{(\cat{S} \bsl \cat{NP})/(\cat{S} \bsl \cat{NP}):\lambda x.\lambda y.\mathrm{to}_{0}^{0}(x\;y)}\inference[<]{\inference[>]{\inference{\token{be}}{(\cat{S} \bsl \cat{NP})/(\cat{S} \bsl \cat{NP}):\lambda x.x}\inference{\token{fine}}{\cat{S} \bsl \cat{NP}:\lambda x.(x_{\circ 6})}}{\cat{S} \bsl \cat{NP}:\lambda x.(x_{\circ 6})}\inference[>]{\inference{\token{for}}{((\cat{S} \bsl \cat{NP}) \bsl (\cat{S} \bsl \cat{NP}))/\cat{NP}:\lambda x.\lambda y.\lambda z.\mathrm{for}_{0}^{0}(y\;x, z)}\inference[>]{\inference{\token{our}}{\cat{NP}/\cat{N}:\lambda x.\mathrm{our}_{0}^{0}(x)}\inference{\token{needs}}{\cat{N}:\mathrm{need}_{0}}}{\cat{NP}:\mathrm{our}_{0}^{0}(\mathrm{need}_{0})}}{(\cat{S} \bsl \cat{NP}) \bsl (\cat{S} \bsl \cat{NP}):\lambda y.\lambda z.\mathrm{for}_{0}^{0}(y\;\mathrm{our}_{0}^{0}(\mathrm{need}_{0}), z)}}{\cat{S} \bsl \cat{NP}:\lambda z.\mathrm{for}_{0}^{0}(\mathrm{our}_{6}^{0}(\mathrm{need}_{0}), z)}}{\cat{S} \bsl \cat{NP}:\lambda y.\mathrm{to}_{0}^{0}(\mathrm{for}_{0}^{0}(\mathrm{our}_{6}^{0}(\mathrm{need}_{0}), y))}}{\cat{NP} \bsl \cat{NP}:\lambda y.\mathrm{to}_{0}^{0}(\mathrm{for}_{0}^{0}(\mathrm{our}_{6}^{0}(\mathrm{need}_{0}), y))}}{\cat{NP}:\mathrm{to}_{0}^{0}(\mathrm{for}_{0}^{0}(\mathrm{our}_{6}^{0}(\mathrm{need}_{0}), \mathrm{service}_{0}))}}{\cat{S} \bsl \cat{NP}:\lambda y.\mathrm{find}_{0}^{0}(\mathrm{to}_{0}^{0}(\mathrm{for}_{0}^{0}(\mathrm{our}_{6}^{0}(\mathrm{need}_{0}), \mathrm{service}_{0})), y)}}{\cat{S}:\mathrm{find}_{0}^{0}(\mathrm{to}_{0}^{0}(\mathrm{for}_{0}^{0}(\mathrm{our}_{6}^{0}(\mathrm{need}_{0}), \mathrm{service}_{0})), \mathrm{we}_{0})}
$$}
